Dafny/W13.dfy
@@ -1,0 +1,245 @@
+/** Abstract Syntax Trees for Arithmetic Expressions
+
+Recall the definition from Rocq:
+Inductive aexp := 
+| ANum (n:nat)
+| AVar (v:string)
+| APlus (a1 a2: aexp)
+| AMult (a1 a2: aexp)
+| AMinus (a1 a2: aexp).
+
+ */
+
+datatype Expr = Const(n:nat)
+| Var(v:string)
+| Node(op: Op, args: List<Expr>)
+
+datatype Op = Add | Mul
+
+datatype List<T> = Nil | Cons(head: T, tail: List<T>)
+
+function Eval(e : Expr, env : map<string,nat>) : nat
+    decreases e
+{
+    match e
+    case Const(n) => n
+    case Var(s) => if s in env.Keys then env[s] else 0
+    case Node(op,args) => EvalList(args, op, env)
+}
+
+function EvalList(args: List<Expr>, op: Op, env: map<string,nat>):nat
+    decreases args
+{
+    match args
+    case Nil => if op == Add then 0 else 1
+    case Cons(h,t) => 
+        var n1,n2 := Eval(h,env), EvalList(t, op, env); 
+            // var bindings inside expressions can be thought of as let expressions.
+        if op == Add then n1 + n2 else n1 * n2 
+}
+
+/** For mutually recursive functions, the termination argument requires the decreases parameter of every call to be decreasing.
+
+For the call from Eval to EvalList:
+Node(op,args) [parameter e of Eval]  > args [parameter args of EvalList]
+
+For the call from EvalList to Eval:
+Cons(h,t) [parameter args of EvalList] > h [parameter e of Eval]
+
+For the call from EvalList to EvalList:
+Cons(h,t) [parameter args of EvalList] > t [parameter args of Eval]
+ */
+
+/** We can enforce a requirement that evaluation of an expression is only possible if its variables have been assigned a value in the environment*/
+
+module EvalWithGoodEnv{
+
+datatype Expr = Const(n:nat)
+| Var(v:string)
+| Node(op: Op, args: List<Expr>)
+
+datatype Op = Add | Mul
+
+datatype List<T> = Nil | Cons(head: T, tail: List<T>)
+
+
+function Eval(e : Expr, env : map<string,nat>) : nat
+    requires GoodEnv(env,e)
+    decreases e
+{
+    match e
+    case Const(n) => n
+    case Var(s) => env[s]
+    case Node(op,args) => EvalList(args, op, env)
+}
+
+function EvalList(args: List<Expr>, op: Op, env: map<string,nat>):nat
+    requires GoodEnvList(env, args)
+    decreases args
+{
+    match args
+    case Nil => if op == Add then 0 else 1
+    case Cons(h,t) => 
+        var n1,n2 := Eval(h,env), EvalList(t, op, env);
+        if op == Add then n1 + n2 else n1 * n2 
+}
+
+predicate GoodEnv(env: map<string,nat>, e: Expr){
+    match e
+    case Var(s) => if s in env.Keys then true else false
+    case Node(op,args) => GoodEnvList(env,args)
+    case _ => true
+}
+
+predicate GoodEnvList(env: map<string,nat>, el: List<Expr>){
+    match el
+    case Nil => true
+    case Cons(h,t) => GoodEnv(env,h) && GoodEnvList(env,t)
+}
+}
+
+/** Lemmas and Proofs */
+
+/** Suppose we want to express that the following function always returns a value greater than its argument */
+function More(x: int): int {
+    if x <= 0 then 1 else More(x - 2) + 3
+}
+
+/** A lemma is similar to a method: it has parameters, a pre-condition/post-condition, as well a body.
+- The logical assertion made by the lemma is its post-condition.
+- A lemma can be called by any other method, in which case the caller can assume the post-condition of the lemma. */
+
+lemma Increasing(x: int)
+    ensures x < More(x)
+{
+
+}
+
+method ExampleMore(a: int) {
+    var b := More(a);
+    var c := More(b);
+    assert 2 <= c - a;
+}
+
+method ExampleLemmaUse(a: int) {
+    var b := More(a);
+    var c := More(b);
+    Increasing(a);
+    Increasing(b);
+    assert 2 <= c - a;
+}
+
+lemma {:induction false} Increasing_2(x: int)
+    ensures x < More(x)
+{
+    if x <= 0 { // this case verifies automatically
+    } else { // this case does not verify automatically
+      Increasing_2(x-2);   // this establishes that x-2 < More(x-2)
+    }
+}
+
+lemma Increasing_wrong(x: int)
+    ensures x < More(x)
+{
+    Increasing_wrong(x);
+}
+/** The proof of Increasing_2 as a decorated program:
+
+lemma {:induction false} Increasing(x: int)
+    ensures x < More(x)
+{
+    { { true } }
+    if x <= 0 {
+        { { x <= 0 } }
+        { { x <= 0 && More(x) == 1 } } // def. More for x <= 0
+        { { x < More(x) } }
+    } else {
+        { { 0 < x } }
+        { { 0 < x && More(x) == More(x - 2) + 3 } } // def. More for 0 < x
+        Increasing(x - 2); // induction hypothesis
+        { { 0 < x && More(x) == More(x - 2) + 3 &&
+        x - 2 < More(x - 2) } }
+        { { More(x) == More(x - 2) + 3 &&
+        x + 1 < More(x - 2) + 3 } }
+        { { x + 1 < More(x) } }
+        { { x < More(x) } }
+    }
+    { { x < More(x) } }
+}
+
+ */
+
+lemma {:induction false} Increasing_verbose(x: int)
+    ensures x < More(x)
+{
+    if x <= 0 {
+        assert More(x) == 1; // def. More for x <= 0
+    } else {
+        assert More(x) == More(x - 2) + 3; // def. More for 0 < x
+        Increasing_verbose(x - 2); // induction hypothesis
+        assert x - 2 < More(x - 2); // what we get from the recursive call
+        assert x + 1 < More(x - 2) + 3; // add 3 to each side
+        assert x + 1 < More(x); // previous line and def. More above
+    }
+}
+
+function Reduce(m: nat, x: int): int {
+    if m == 0 then x else Reduce(m / 2, x + 1) - m
+}
+
+lemma {:induction false} Decreasing(m:nat, x:int)
+    ensures Reduce(m,x) <= x
+{
+    if m == 0 
+    {
+        calc{
+            Reduce(m,x) == x;
+            ==>
+            Reduce(m,x) <= x;
+        }
+
+    }
+    else
+    {
+        calc{
+            true;
+             ==> {Decreasing(m/2,x+1);}
+            Reduce(m/2,x+1) <= x + 1;
+             ==> {assert(m >= 1);}
+            Reduce(m/2,x+1) <= x + m; 
+             ==>
+            Reduce(m/2,x+1) - m <= x;
+             ==> {assert(Reduce(m,x) == Reduce(m/2,x+1)-m);}
+            Reduce(m,x) <= x;
+        }
+    }
+}
+
+lemma {:induction false} ReduceLowerBound(m: nat, x: int)
+    ensures x - 2 * m <= Reduce(m, x)
+{
+    if m == 0 
+    {
+        calc{
+            Reduce(m,x) == x;
+            ==>
+            x - 2 * m <= Reduce(m,x);
+        }
+    }
+    else
+    {
+        calc{
+            true; 
+            ==> {ReduceLowerBound(m/2,x+1);}
+            x + 1 - 2 * (m / 2) <= Reduce(m/2,x+1);
+            ==> {assert (2 * (m / 2) <= m);}
+            x + 1 - m <= Reduce(m/2,x+1);
+            ==> {assert (x - m <= x + 1 - m);}
+            x - m <= Reduce(m/2,x+1);
+            ==>
+            x - 2 * m <= Reduce(m/2,x+1) - m;
+            ==>
+            x - 2 * m <= Reduce(m,x);
+        }
+    }
+}
